NewFSet -> FSet + ISet removal
- Predicates and predicate operations replace ISet and ISet
  operations.

- A new theory Finite defines an 'is_finite P' predicate that holds if
  there exists a unique list whose membership predicate coincides with
  P.  We are still peg-legging our way between sums over fsets and sums
  over lists throughout the libraries. In particular, the fel still sums
  over a set.

Sign-Off: François Dupressoir

src/ecCoreLib.ml
@@ -106,7 +106,7 @@ end
 (* -------------------------------------------------------------------- *)
 module CI_FSet = struct
   let p_FSet = EcPath.pqname p_top "FSet"
-  let p_fset = EcPath.pqname p_FSet "set"
+  let p_fset = EcPath.pqname p_FSet "fset"
 end
 
 (* -------------------------------------------------------------------- *)
