theories/Sum.ec
@@ -5,32 +5,34 @@
  * Distributed under the terms of the CeCILL-B-V1 license
  * -------------------------------------------------------------------- *)
 
-require import FSet. import Interval.
-require import Int.
-require import Real.
-require import Monoid.
+require import List FSet Int Real Monoid.
 
 (* temporary workaround *)
-op intval : int -> int -> int set = interval.
+op intval : int -> int -> int fset = fun (i j:int) =>
+  oflist (List.Iota.iota_ i (j - i + 1)).
 
 lemma intval_def i i1 i2:
-  mem i (intval i1 i2)  <=> (i1<= i /\ i <= i2)
+  mem (intval i1 i2) i <=> (i1<= i /\ i <= i2)
 by [].
 
 lemma intval_card_0 i1 (i2 : int):
   i1 <= i2 =>
-  card (intval i1 i2) = i2 - i1 + 1
-by [].
+  card (intval i1 i2) = i2 - i1 + 1.
+proof.
+  move=> le_i1_i2; rewrite cardE.
+  rewrite -(perm_eq_size (iota_ i1 (i2 - i1 + 1))) 2:size_iota 2:smt.
+  by rewrite -(undup_id (iota_ i1 (i2 - i1 + 1))) 1:iota_uniq// /intval oflistK// iota_uniq//.
+qed.
 
 lemma intval_card_1 (i1 i2:int):
   i2 < i1 => card (intval i1 i2) = 0
 by [].
 
-op int_sum: (int -> real) -> int set -> real = Mrplus.sum.
+op int_sum: (int -> real) -> int fset -> real = Mrplus.sum.
 
 pred is_cnst (f : int -> 'a) = forall i1 i2, f i1 = f i2.
 
-lemma int_sum_const (f : int -> real) (s: int set):
+lemma int_sum_const (f : int -> real) (s: int fset):
   is_cnst f => int_sum f s = (card s)%r * f 0.
 proof strict.
 by intros=> is_cnst;
