theories/core/FMap.ec
@@ -40,38 +40,38 @@ axiom map_ext (m1 m2:('a,'b) map):
   m1 == m2 => m1 = m2.
 
 (** Domain *)
-op dom: ('a,'b) map -> 'a set.
+op dom: ('a,'b) map -> 'a fset.
 
 axiom mem_dom (m:('a,'b) map) x:
-  mem x (dom m) <=> m.[x] <> None.
+  mem (dom m) x <=> m.[x] <> None.
 
-lemma dom_empty: dom empty<:'a,'b> = FSet.empty.
+lemma dom_empty: dom empty<:'a,'b> = fset0.
 proof.
-apply set_ext=> x.
-by rewrite mem_dom get_empty mem_empty.
+  apply fsetP=> x.
+  by rewrite mem_dom get_empty in_fset0.
 qed.
 
-lemma empty_dom (m:('a,'b) map): dom m = FSet.empty => m = empty<:'a,'b>.
+lemma empty_dom (m:('a,'b) map): dom m = fset0 => m = empty<:'a,'b>.
 proof.
   move=> dom_empty; apply map_ext=> x.
   smt.
 qed.
 
 (** Range *)
-op rng: ('a,'b) map -> 'b set.
+op rng: ('a,'b) map -> 'b fset.
 
 axiom mem_rng (m:('a,'b) map) y:
-  mem y (rng m) <=> exists x, m.[x] = Some y.
+  mem (rng m) y <=> exists x, m.[x] = Some y.
 
-lemma rng_empty: rng empty<:'a,'b> = FSet.empty.
+lemma rng_empty: rng empty<:'a,'b> = fset0.
 proof.
-  apply set_ext=> y.
+  apply fsetP=> y.
   by rewrite mem_rng; smt.
 qed.
 
 (** Less defined than *)
 pred (<=) (m1 m2:('a,'b) map) = forall x,
-  mem x (dom m1) =>
+  mem (dom m1) x =>
   m1.[x] = m2.[x].
 
 lemma leq_dom (m1 m2:('a,'b) map):
@@ -117,11 +117,11 @@ qed.
 op size (m:('a,'b) map) = card (dom m).
 
 lemma nosmt size_nneg (m:('a,'b) map): 0 <= size m.
-proof. by rewrite /size card_def List.size_ge0. qed.
+proof. by rewrite /size cardE List.size_ge0. qed.
 
 lemma nosmt size_empty: size empty<:'a,'b> = 0.
 proof.
-by rewrite /size dom_empty card_empty.
+by rewrite /size dom_empty fcards0.
 qed.
 
 lemma nosmt size_leq (m1 m2:('a,'b) map):
@@ -144,16 +144,16 @@ lemma nosmt get_rm_neq (m:('a,'b) map) x x':
 by (rewrite -neqF get_rm=> ->).
 
 lemma dom_rm (m:('a,'b) map) x:
-  dom (rm x m) = rm x (dom m).
+  dom (rm x m) = (dom m) `\` (fset1 x).
 proof.
-apply set_ext=> x'; rewrite mem_dom get_rm mem_rm;
+apply fsetP=> x'; rewrite mem_dom get_rm in_fsetD in_fset1;
 case (x = x').
   by intros=> <-.
   by rewrite eq_sym mem_dom=> ->.
 qed.
 
 lemma rng_rm (m:('a,'b) map) x y:
-  mem y (rng (rm x m)) = (exists x', x <> x' /\ m.[x'] = Some y).
+  mem (rng (rm x m)) y = (exists x', x <> x' /\ m.[x'] = Some y).
 proof.
   rewrite mem_rng eq_iff; split.
     elim=> x'; rewrite get_rm.
@@ -164,30 +164,22 @@ proof.
 qed.
 
 lemma size_rm (m:('a,'b) map) x:
-  size (rm x m) = if mem x (dom m) then size m - 1 else size m.
+  size (rm x m) = if mem (dom m) x then size m - 1 else size m.
 proof.
-rewrite /size dom_rm; case (mem x (dom m))=> x_m.
-  by rewrite card_rm_in.
-  by rewrite card_rm_nin.
+  by rewrite /size dom_rm (fcardD1 (dom m) x); case (mem (dom m) x); 1:smt.
 qed.
 
 lemma nosmt size_rm_in (m:('a,'b) map) x:
-  mem x (dom m) =>
+  mem (dom m) x =>
   size (rm x m) = size m - 1.
-proof.
-by rewrite /size dom_rm=> x_m;
-   rewrite card_rm_in.
-qed.
+proof. by rewrite size_rm=> ->. qed.
 
 lemma nosmt size_rm_nin (m:('a,'b) map) x:
-  !mem x (dom m) =>
+  !mem (dom m) x =>
   size (rm x m) = size m.
-proof.
-by rewrite /size dom_rm=> x_m;
-   rewrite card_rm_nin.
-qed.
+proof. by rewrite size_rm=> ->. qed.
 
-lemma rm_nin_id x (m:('a,'b) map): !mem x (dom m) => rm x m = m.
+lemma rm_nin_id x (m:('a,'b) map): !mem (dom m) x => rm x m = m.
 proof.
   move=> x_notin_m.
   apply map_ext=> x'; rewrite get_rm.
@@ -219,40 +211,39 @@ proof.
 qed.
 
 lemma dom_set (m:('a,'b) map) x y:
-  dom (m.[x <- y]) = add x (dom m).
+  dom (m.[x <- y]) = (dom m) `|` fset1 x.
 proof.
-apply set_ext=> x'; rewrite mem_add; case (x = x').
+apply fsetP=> x'; rewrite in_fsetU in_fset1; case (x = x').
   by move=> <-; rewrite mem_dom get_set.
   by rewrite -neqF=> x_x'; rewrite (eq_sym x') 2!mem_dom get_set_neq ?x_x'.
 qed.
 
 lemma nosmt dom_set_in (m:('a,'b) map) x y:
-  mem x (dom m) =>
+  mem (dom m) x =>
   dom (m.[x <- y]) = dom m.
 proof.
-by move=> x_m; rewrite dom_set -add_in_id.
+  rewrite dom_set fsetP=> x_in_m x'.
+  by rewrite in_fsetU in_fset1; move: x_in_m; case (x' = x)=> [<<-|].
 qed.
 
 lemma nosmt dom_set_nin (m:('a,'b) map) x y x':
-  !mem x' (dom m) =>
-  (mem x' (dom (m.[x <- y])) <=> x' = x).
-proof.
-by rewrite dom_set mem_add=> ->.
-qed.
+  !mem (dom m) x' =>
+  (mem (dom (m.[x <- y])) x' <=> x' = x).
+proof. by rewrite dom_set in_fsetU in_fset1=> ->. qed.
 
 lemma mem_dom_set y x (m:('a,'b) map) x':
-  mem x' (dom m.[x <- y]) <=> (mem x' (dom m) \/ x' = x).
-proof. by rewrite dom_set mem_add. qed.
+  mem (dom m.[x <- y]) x' <=> (mem (dom m) x' \/ x' = x).
+proof. by rewrite dom_set in_fsetU in_fset1. qed.
 
 lemma dom_set_stable (m:('a,'b) map) x y x':
-  mem x' (dom m) => mem x' (dom m.[x <- y]).
+  mem (dom m) x' => mem (dom m.[x <- y]) x'.
 proof. by rewrite mem_dom_set=> H; left. qed.
 
 lemma rng_set (m:('a,'b) map) x y:
-  rng (m.[x <- y]) = add y (rng (rm x m)).
+  rng (m.[x <- y]) = (rng (rm x m)) `|` fset1 y.
 proof.
-  apply set_ext=> y'.
-  rewrite mem_add !mem_rng; split.
+  apply fsetP=> y'.
+  rewrite in_fsetU in_fset1 !mem_rng; split.
     elim=> x'; rewrite get_set; case (x = x').
       by move=> H {H x'}; move=> y_eq_y'; apply someI in y_eq_y'; rewrite eq_sym; right.
       by move=> x_neq_x' mx'_y'; left; exists x'; rewrite get_rm_neq.
@@ -261,28 +252,20 @@ proof.
 qed.
 
 lemma size_set (m:('a,'b) map) x y:
-  size m.[x <- y] = if mem x(dom m) then size m else size m + 1.
+  size m.[x <- y] = if mem (dom m) x then size m else size m + 1.
 proof.
-rewrite /size dom_set; case (mem x (dom m))=> x_m.
-  by rewrite card_add_in.
-  by rewrite card_add_nin.
+rewrite /size dom_set; case (mem (dom m) x)=> x_m; smt.
 qed.
 
 lemma nosmt size_set_in (m:('a,'b) map) x y:
-  mem x (dom m) =>
+  mem (dom m) x =>
   size m.[x <- y] = size m.
-proof.
-by rewrite /size dom_set=> x_m;
-   rewrite card_add_in.
-qed.
+proof. by rewrite size_set; smt. qed.
 
 lemma nosmt size_set_nin (m:('a,'b) map) x y:
-  !mem x (dom m) =>
+  !mem (dom m) x =>
   size m.[x <- y] = size m + 1.
-proof.
-by rewrite /size dom_set=> x_m;
-   rewrite card_add_nin.
-qed.
+proof. by rewrite size_set=> ->. qed.
 
 lemma set_set (m:('a,'b) map) x x' y y':
   m.[x <- y].[x' <- y'] = if x = x' then m.[x' <- y']
@@ -309,7 +292,7 @@ lemma set_set_neq (m:('a,'b) map) x x' y y':
 by (rewrite -neqF set_set=> ->).
 
 lemma set_same (x:'a) (m:('a,'b)map):
-   mem x (dom m) =>
+   mem (dom m) x =>
    m.[x <- oget m.[x]] = m.
 proof.
   by move=> Hm; apply map_ext; smt.
@@ -317,7 +300,7 @@ qed.
 
 (* all and allb *)
 pred all (p:'a -> 'b -> bool) (m:('a,'b) map) = forall x,
-  mem x (dom m) =>
+  mem (dom m) x =>
   p x (oget m.[x]).
 
 op allb: ('a -> 'b -> bool) -> ('a,'b) map -> bool.
@@ -327,7 +310,7 @@ axiom allb_all (p:'a -> 'b -> bool) (m:('a,'b) map):
 
 (* exist and existb *)
 pred exist (p:'a -> 'b -> bool) (m:('a,'b) map) = exists x,
-  mem x (dom m) /\ p x (oget m.[x]).
+  mem (dom m) x /\ p x (oget m.[x]).
 
 op existb: ('a -> 'b -> bool) -> ('a,'b) map -> bool.
 
@@ -353,7 +336,7 @@ lemma all_set_all_in (p:'a -> 'b -> bool) (m:('a,'b) map) x y:
 proof.
 intros=> p_m p_xy a; case (x = a).
   by intros=> <- _; rewrite get_set_eq oget_some.
-  intros=> a_x; rewrite get_set_neq // dom_set mem_add (_: (a = x) = false) 1:(eq_sym a) 1:neqF //= => a_m.
+  intros=> a_x; rewrite get_set_neq // dom_set in_fsetU in_fset1 (_: (a = x) = false) 1:(eq_sym a) 1:neqF //= => a_m.
   by rewrite p_m.
 qed.
 
@@ -365,7 +348,7 @@ axiom find_nin (p:'a -> 'b -> bool) m:
 
 axiom find_cor (p:'a -> 'b -> bool) m x:
   find p m = Some x =>
-  mem x (dom m) /\ p x (oget m.[x]).
+  mem (dom m) x /\ p x (oget m.[x]).
 
 lemma find_in (p:'a -> 'b -> bool) (m:('a,'b) map):
   exist p m <=> find p m <> None.
@@ -388,7 +371,7 @@ qed.
 
 lemma find_unique x' p (m:('a,'b) map):
   (forall x, p x (oget m.[x]) => x = x') =>
-  mem x' (dom m) =>
+  mem (dom m) x' =>
   p x' (oget m.[x']) =>
   find p m = Some x'.
 proof.
@@ -406,7 +389,7 @@ axiom find1_nin (p:'a -> bool) (m:('a,'b) map):
 
 axiom find1_cor (p:'a -> bool) (m:('a,'b) map) x:
   find1 p m = Some x =>
-  mem x (dom m) /\ p x.
+  mem (dom m) x /\ p x.
 
 lemma find1_in (p:'a -> bool) (m:('a,'b) map):
   exist (fun x y, p x) m <=> find1 p m <> None.
@@ -427,7 +410,7 @@ lemma filter_empty (f:'a -> 'b -> bool):
 proof. by apply map_ext=> x;smt. qed.
 
 lemma nosmt get_filter_nin f (m:('a,'b) map) x:
-  !mem x (dom m) =>
+  !mem (dom m) x =>
   (filter f m).[x] = m.[x].
 proof.
 by rewrite get_filter mem_dom /= => ->.
@@ -436,7 +419,7 @@ qed.
 lemma dom_filter f (m:('a,'b) map):
   dom (filter f m) = filter (fun x, f x (oget m.[x])) (dom m).
 proof.
-by apply set_ext=> x; rewrite mem_dom get_filter mem_filter mem_dom /=;
+by apply fsetP=> x; rewrite mem_dom get_filter in_filter mem_dom /=;
    case (f x (oget m.[x])).
 qed.
 
@@ -445,9 +428,9 @@ lemma dom_filter_fst f (m:('a,'b) map):
 proof. by apply/(dom_filter (fun x (y : 'b) => f x)). qed.
 
 lemma mem_dom_filter f (m:('a,'b) map) x:
-  mem x (dom (filter f m)) =>
-  mem x (dom m) /\ f x (oget m.[x])
-by (rewrite dom_filter mem_filter).
+  mem (dom (filter f m)) x =>
+  mem (dom m) x /\ f x (oget m.[x])
+by (rewrite dom_filter in_filter).
 
 lemma leq_filter f (m:('a,'b) map):
   filter f m <= m.
@@ -494,7 +477,7 @@ by [].
 
 lemma eq_except_eq (m1 m2:('a,'b) map) x x':
   eq_except m1 m2 x =>
-  mem x' (dom m1) <=> !mem x' (dom m2) =>
+  mem (dom m1) x' <=> !mem (dom m2) x' =>
   x = x'
 by [].
 
@@ -504,7 +487,7 @@ lemma eq_except_set1_eq (m1 m2:('a,'b) map) x y:
 by [].
 
 lemma eq_except_in_dom (m1 m2:('a, 'b) map) (x y:'a) :
-  eq_except m1 m2 x => x <> y => (mem y (dom m1) <=> mem y (dom m2))
+  eq_except m1 m2 x => x <> y => (mem (dom m1) y <=> mem (dom m2) y)
 by [].
 
 lemma eq_except_set2 (m1 m2:('a,'b) map) x x' y1 y2:
@@ -535,10 +518,10 @@ proof. by apply map_ext;intros x';case (x = x');smt. qed.
 
 lemma dom_map (f:'b -> 'c) (m:('a,'b) map):
    dom (map f m) = dom m.
-proof. by apply set_ext=> x; rewrite !mem_dom get_map; case (m.[x]). qed.
+proof. by apply fsetP=> x; rewrite !mem_dom get_map; case (m.[x]). qed.
 
 lemma mem_rng_map (f:'b -> 'c) (m:('a,'b) map) (y:'c):
-  mem y (rng (map f m)) = exists x, omap f m.[x] = Some y
+  mem (rng (map f m)) y = exists x, omap f m.[x] = Some y
 by [].
 
 op mapi: ('a -> 'b -> 'c) -> ('a,'b) map -> ('a,'c) map.
@@ -550,33 +533,26 @@ axiom get_mapi (f:'a -> 'b -> 'c) (m:('a,'b) map) (x:'a):
 lemma leq_card_rng_dom (m:('a,'b) map):
   card (rng m) <= card (dom m).
 proof.
-  move: {-2}m (Logic.eq_refl (dom m)).
-  elim/set_ind (dom m)=> {m} [|x s x_notin_s ih m].
-    by move=> m /empty_dom ->; rewrite rng_empty dom_empty !card_empty.
-    move=> m_addx.
+  elim/fset_ind (dom m) {-2}m (Logic.eq_refl (dom m))=> {m} [|x s x_notin_s ih m dom_m].
+    by move=> m /empty_dom ->; rewrite rng_empty dom_empty !fcards0.
     cut ->: m = (rm x m).[x <- oget m.[x]].
       by apply map_ext=> x0; rewrite get_set; smt.
     rewrite rng_set.
     cut ->: rm x (rm x m) = (rm x m).
       by apply map_ext=> x0; smt.
-    cut dom_rmxm: dom (rm x m) = s by smt.
-    case (mem (oget m.[x]) (rng (rm x m)))=> [mx_in_rmxm | mx_notin_rmxm].
-      rewrite card_add_in // dom_set card_add_nin dom_rmxm //.
-      cut: card (rng (rm x m)) <= card (dom (rm x m)); last smt.
-      by apply ih.
-      rewrite dom_set !card_add_nin ?dom_rmxm //.
-      cut: card (rng (rm x m)) <= card (dom (rm x m)); last smt.
-      by apply ih.
+    by case (mem (dom m) x); smt.
 qed.
 
 lemma endo_dom_rng (m:('a,'a) map):
-  (exists x, !mem x (dom m)) =>
-  exists x, !mem x (rng m).
+  (exists x, !mem (dom m) x) =>
+  exists x, !mem (rng m) x.
 proof.
   elim=> x x_notin_m.
-  cut: 0 < card (sub (add x (dom m)) (rng m)); last smt ml=100.
-  apply sub_card.
-  rewrite card_add_nin //.
+  cut: 0 < card (((dom m) `|` fset1 x) `\` (rng m)); last smt.
+  rewrite fcardD !fcardU !fcard1.
+  have ->: dom m `&` fset1 x = fset0.
+    by apply/fsetP=> x'; rewrite in_fsetI in_fset1 in_fset0 /=; case (x' = x).
+  rewrite !fcards0 //=.
   smt.
 qed.    
 
