theories/newth/Finite.ec
@@ -1,0 +1,76 @@
+require import Pred List.
+
+pred is_finite (p : 'a -> bool) =
+  exists s,
+       uniq s
+    /\ (forall x, mem s x <=> p x).
+
+(** Not sure how to have this expressed without axioms. **)
+op to_seq: ('a -> bool) -> 'a list.
+axiom to_seq_finite (P : 'a -> bool):
+  is_finite P =>
+     uniq (to_seq P)
+  /\ (forall x, mem (to_seq P) x <=> P x).
+
+lemma uniq_to_seq (P : 'a -> bool):
+  is_finite P =>
+  uniq (to_seq P).
+proof. by move=>/to_seq_finite [-> _]. qed.
+
+lemma mem_to_seq (P : 'a -> bool) x:
+  is_finite P =>
+  mem (to_seq P) x <=> P x.
+proof. by move=>/to_seq_finite [_ ->]. qed.
+
+(* Finite sets can be obtained by union, intersection and difference
+ * of empty and singleton sets. Finiteness is closed under inclusion.  *)
+lemma finite0: is_finite pred0<:'a>.
+proof. by exists []. qed.
+
+lemma finite1 (x : 'a): is_finite (pred1 x).
+proof. by exists [x]. qed.
+
+lemma finite_leq (B A : 'a -> bool):
+  A <= B => is_finite B =>
+  is_finite A.
+proof.
+  move=> le_A_B [wB] [uniq_wB wB_univ].
+  exists (filter A wB); split=> [|x].
+    exact/filter_uniq.
+  rewrite mem_filter wB_univ.
+  by case (A x)=> //=; exact/le_A_B.
+qed.
+
+lemma finiteU (A B : 'a -> bool):
+  is_finite A => is_finite B =>
+  is_finite (predU A B).
+proof.
+  move=> [wA] [uniq_wA wA_univ] [wB] [uniq_wB wB_univ].
+  exists (undup (wA ++ wB)); split=> [|x].
+    exact/undup_uniq.
+  by rewrite /predU mem_undup mem_cat wA_univ wB_univ.
+qed.
+
+lemma finiteIl (A B : 'a -> bool):
+  is_finite A =>
+  is_finite (predI A B).
+proof.
+  move=> fin_A; apply/(finite_leq A)=> //=.
+  exact/predIsubpredl.
+qed.
+
+lemma finiteIr (A B : 'a -> bool):
+  is_finite B =>
+  is_finite (predI A B).
+proof.
+  move=> fin_B; apply/(finite_leq B)=> //=.
+  exact/predIsubpredr.
+qed.
+
+lemma finiteD (A B : 'a -> bool):
+  is_finite A =>
+  is_finite (predD A B).
+proof.
+  move=> fin_A; apply/(finite_leq A)=> //= x.
+  by rewrite /predD.
+qed.
