theories/newth/distributions/Mu_mem.ec
@@ -1,0 +1,86 @@
+require import Int Real List FSet Distr.
+
+lemma mu_mem_le (s:'a fset): forall (d:'a distr) (bd:real),
+  (forall (x : 'a), mem s x => mu d (pred1 x) <= bd) =>
+  mu d (mem s) <= (card s)%r * bd.
+proof.
+  elim/fset_ind s=> [d bd mu_bound|x s x_notin_s ih d bd mu_bound].
+    by rewrite (mu_eq d _ pred0) 2:mu_false 2:fcards0 // => x; rewrite inE.
+  rewrite fcardUI_indep 1:fsetP 2:fcard1.
+    by move=> x0; rewrite !inE; split=> [[h ->>]|].
+  rewrite Int.CommutativeGroup.Comm.Comm Add Mul_distr_r /=.
+  rewrite (mu_eq d _ (predU (pred1 x) (mem s))).
+    by move=> z; rewrite !inE orbC.
+  rewrite mu_disjoint.
+    by rewrite /predI /pred1 /pred0=> z [->].
+  rewrite addleM 1:mu_bound // 1:!inE //.
+  by apply ih=> z z_in_s; rewrite mu_bound // !inE; left.
+qed.
+
+lemma mu_mem_ge (s:'a fset): forall (d:'a distr) (bd:real),
+  (forall (x : 'a), mem s x => mu d (pred1 x) >= bd) =>
+  mu d (mem s) >= (card s)%r * bd.
+proof.
+  elim/fset_ind s=> [d bd mu_bound|x s x_notin_s ih d bd mu_bound].
+    by rewrite (mu_eq d _ pred0) 2:mu_false 2:fcards0 2:-le_ge // => x; rewrite inE.
+  rewrite fcardUI_indep 1:fsetP 2:fcard1.
+    by move=> x0; rewrite !inE; split=> [[h ->>]|].
+  rewrite Int.CommutativeGroup.Comm.Comm Add Mul_distr_r /=.
+  rewrite (mu_eq d _ (predU (pred1 x) (mem s))).
+    by move=> z; rewrite !inE orbC.
+  rewrite mu_disjoint.
+    by rewrite /predI /pred1 /pred0=> z [->].
+  rewrite addgeM 1:mu_bound // 1:!inE //.
+  by apply ih=> z z_in_s; rewrite mu_bound // !inE; left.
+qed.
+
+lemma mu_mem (s:'a fset): forall (d:'a distr) (bd:real),
+  (forall (x : 'a), mem s x => mu d (pred1 x) = bd) =>
+  mu d (mem s) = (card s)%r * bd.
+proof.
+  move=> d bd mu_cnst; rewrite eq_le_ge; split.
+    by apply mu_mem_le=> x h; rewrite mu_cnst.
+  by apply mu_mem_ge=> x h; rewrite mu_cnst // -le_ge.
+qed.
+
+lemma mu_mem_card (l:'a list) (d:'a distr) (bd:real):
+  (forall (x : 'a), mem l x => mu d (pred1 x) = bd) =>
+  mu d (mem l) = (card (oflist l))%r * bd.
+proof.  
+  move=> mu_cnst; rewrite (mu_eq _ _ (mem (oflist l))).
+    by move=> x; rewrite mem_oflist.
+  by apply mu_mem=> x; rewrite mem_oflist=> /mu_cnst.
+qed.
+
+lemma mu_mem_le_card (l:'a list) (d:'a distr) (bd:real):
+  (forall (x : 'a), mem l x => mu d (pred1 x) <= bd) =>
+  mu d (mem l) <= (card (oflist l))%r * bd.
+proof.  
+  move=> mu_bound; rewrite (mu_eq _ _ (mem (oflist l))).
+    by move=> x; rewrite mem_oflist.
+  by apply mu_mem_le=> x; rewrite mem_oflist=> /mu_bound.
+qed.
+
+lemma mu_mem_ge_card (l:'a list) (d:'a distr) (bd:real):
+  (forall (x : 'a), mem l x => mu d (pred1 x) >= bd) =>
+  mu d (mem l) >= (card (oflist l))%r * bd.
+proof.  
+  move=> mu_bound; rewrite (mu_eq _ _ (mem (oflist l))).
+    by move=> x; rewrite mem_oflist.
+  by apply mu_mem_ge=> x; rewrite mem_oflist=> /mu_bound.
+qed.
+
+lemma mu_mem_le_size (l:'a list) (d:'a distr) (bd:real):
+  (forall (x : 'a), mem l x => mu d (pred1 x) <= bd) =>
+  mu d (mem l) <= (size l)%r * bd.
+proof.
+  case l=> [//=|x l mu_bound].
+    by rewrite (mu_eq _ _ pred0) // mu_false.
+  have le0_mu: Real.zero <= bd.
+    by have := mu_bound x _=> //; smt.
+  move: (x::l) mu_bound=> {x l} l mu_bound.
+  apply (Trans _ ((card (oflist l))%r * bd)).
+    exact/(mu_mem_le_card l d bd mu_bound).
+  rewrite cardE -(perm_eq_size (undup l)) 1:oflistK// CompatOrderMult //.
+  by rewrite from_intMle size_undup.
+qed.
